\section{Proof of Lemmas}
\label{sec:proof}

\begin{lemma}
\label{lem:okPreserved}
If \(\OK_n(P)\) and \(P \xlongrightarrow{\rho} P'\), then
\begin{itemize}
\item \(\OK_{n-1}(P')\) if \(\rho = \Malloc\),
\item \(\OK_{n+1}(P')\) if \(\rho = \Free\),
\item \(\OK_n(P')\) if \(\rho = \sassx\) \( \mbox{ or } \rho = \sassxn \)
\item \(\OK_n(P')\) if \(\rho = \Startconst\) \( \mbox{ or } \rho = \Endconst \)
\item \(\OK_n(P')\) if \(\rho = \tau\).
\end{itemize}
\end{lemma}

\begin{proof}
Case analysis on \(P \xlongrightarrow{\rho} P'\).

\begin{itemize}

\item Case $P = \TSKIP;P'$ and \(\TSKIP;P' \xlongrightarrow{\tau} P'\)

  We need to prove \(\OK_n(P')\).  Assume that \(\OK_n(P')\) does not
  hold. Then, we have \(\TSKIP;P' \xlongrightarrow{\tau} P'
  \xlongrightarrow{\sigma} Q\) such that \(\sharp_{m}(\sigma) -
  \sharp_{f}(\sigma) > n\) for some \(\sigma\).  From the definition
  of \(\OK_n(P)\), we have \(\sharp_m(\tau\sigma) - \sharp_f(\tau
  \sigma) \le n \).  From the definition of \(\sharp_\rho(\sigma)\),
  we get \(\sharp_m(\tau) + \sharp_m(\sigma) - \sharp_f(\tau) -
  \sharp_f(\sigma) \le n\) that is equivalent to \(\sharp_m(\sigma) -
  \sharp_f(\sigma) \le n\), which is contradiction.

\item Case $P = \Malloc$ and \(\Malloc \xlongrightarrow{\Malloc} \TSKIP\)

  We need to prove \(\OK_{n-1}(\TSKIP)\).  From the definition of
  \(\OK_n(P)\), we have that \(\OK_{n-1}(\TSKIP)\) holds if, for any
  \(P'\), if \(\TSKIP \xlongrightarrow{\sigma} P'\) then
  \(\sharp_m(\sigma) - \sharp_f(\sigma) \le n - 1\). There is no such \(P'\) s.t. \(\TSKIP
  \xlongrightarrow{\sigma} P'\), therefore, \(\OK_{n-1}(\TSKIP)\) holds.

\item Case $P = \Free$ and \(\Free \xlongrightarrow{\Free} \TSKIP\)

    We need to prove \(\OK_{n+1}(\TSKIP)\).  From the definition of
    \(\OK_n(P)\), we have that \(\OK_{n+1}(\TSKIP)\) holds if, for any
    \(P'\), if \(\TSKIP \xlongrightarrow{\sigma} P'\) then
    \(\sharp_m(\sigma) - \sharp_f(\sigma) \le n + 1\). There is no
    such \(P'\) s.t. \(\TSKIP \xlongrightarrow{\sigma} P'\),
    therefore, \(\OK_{n+1}(\TSKIP)\) holds.    

\item Case \( P = (*x)(P_1,P_2) \) and \( (*x)(P_1,P_2) \) \(\xlongrightarrow{\sassx} P_1\)

  We prove \(\OK_n(P_1)\) by contradiction. Assume that
  \(OK_{n}(P_1)\) does not hold.  Then, there exists \(\sigma\) such
  that \( (*x)(P_1,P_2) \xlongrightarrow{\sassx} P_{1}
  \xlongrightarrow{\sigma} Q\) and \(\sharp_{m}(\sigma) -
  \sharp_{f}(\sigma) > n\).  From the definition of \(\OK_n(P)\), we
  have \(\sharp_m(\sassx) + \sharp_m(\sigma) -\sharp_f(\sassx)
  -\sharp_f(\sigma) \le n\).  By the definition of
  \(\sharp_\rho(\sigma)\), we get \(\sharp_m(\sigma) -\sharp_f(\sigma)
  \le n\). Therefore, we get the contradiction.

\item Case \( P = (*x)(P_1,P_2) \) and \( (*x)(P_1,P_2)\xlongrightarrow{\sassxn} P_2\)

  Similar to the case of \( (*x)(P_1,P_2) \xlongrightarrow{\sassx}
  P_1\).

  \item Case \(P = \scon\Sirx P'\) and \( \scon\Sirx P'
    \xlongrightarrow{\Startconst} P';\Endconst \) 

    We prove \( OK_n(P';\Endconst) \) by
    contradiction. Assume that \( OK_n(P';\Endconst) \) does not
    hold, then we have \( \scon\Sirx P' \xlongrightarrow{\Startconst}
    P';\Endconst \xlongrightarrow{\sigma} Q \) such that \(
    \sharp_m(\sigma) - \sharp_f(\sigma) > n \) for some \( \sigma \)
    and \( Q \).  From the definition of \( OK_n(P)\), we have \(
    \sharp_m(\Startconst;\sigma) - \sharp_f(\Startconst;\sigma) \le n
    \), then we get \( \sharp_m(\sigma) - \sharp_f(\sigma) \le n \),
    which is a contradiction.

\item Case \(P = \Endconst \) and \( \Endconst \xlongrightarrow{\Endconst}  0 \)

    We need to prove \( OK_n(0) \). From the definition of \( OK_n(P)
    \), we have that \( OK_n(0) \) holds if, \( \forall \sigma, P'
    \). if \( 0 \xlongrightarrow{\sigma} P' \) and \( \sconst\), then
    \( \sharp_m(\sigma) - \sharp_f(\sigma) \le n \). There is no such
    \(P'\) s.t. \( 0 \xlongrightarrow{\sigma} P' \), therefore, \( OK_n(0)
    \) holds.

\item Case $P = P_{1} + P_{2}$ and \(P_1 + P_2 \xlongrightarrow{\tau} P_1\)

  We prove \(\OK_n(P_1)\) by contradiction.  Assume that
  \(OK_{n}(P_1)\) does not hold.  Then, there exists \(\sigma\) such
  that \(P_{1} + P_{2} \xlongrightarrow{\tau} P_{1}
  \xlongrightarrow{\sigma} Q\) and \(\sharp_{m}(\sigma) -
  \sharp_{f}(\sigma) > n\).  From the definition of \(\OK_n(P)\), we
  have \(\sharp_m(\tau\sigma) -\sharp_f(\tau\sigma) \le n\). Then, we
  have \(\sharp_m(\tau) + \sharp_m(\sigma) - \sharp_f(\tau)
  -\sharp_f(\sigma) \le n\).  By the definition of \(
  \sharp_\rho(\sigma) \), we get \( \sharp_m(\sigma) -\sharp_f(\sigma)
  \le n \). Therefore, we get the contradiction.

\item Case $P = P_{1} + P_{2}$ and \(P_1 + P_2 \xlongrightarrow{\tau} P_2\)

  Similar to the case of \(P_1 + P_2 \xlongrightarrow{\tau} P_1\).

\item Case $P = P_{1};P_{2}$ and \(P_1;P_2 \xlongrightarrow{\rho} P_1';P_2\).

We need to prove \(\OK_{n'}(P_1';P_2)\) where \(n'\) is determined by
\[
   n'=\left\{
   \begin{array}{ll}
     n + 1 & \rho = \Free\\
     n - 1 & \rho = \Malloc\\
     n & \mbox{Otherwise.}
   \end{array}
   \right.
\]
Assume that \(OK_{n'}(P_{1}';P_{2})\) does not hold. Then, there
exists \(\sigma\) such that \(P_{1};P_{2} \xlongrightarrow{\rho}
P_{1}';P_{2} \xlongrightarrow{\sigma} Q\) and \(\sharp_{m}(\sigma) -
\sharp_{f}(\sigma) > n'\).  From the definition of \(\OK_n(P)\), we
have \( \sharp_{m}(\rho\sigma) - \sharp_{f}(\rho\sigma) \le n\); hence
we have \(\sharp_{m}(\rho) + \sharp_{m}(\sigma) - \sharp_{f}(\rho)
-\sharp_{f}(\sigma) \le n\).  From the assumption \(\sharp_{m}(\sigma)
- \sharp_{f}(\sigma) > n'\), we have
\[
n' + \sharp_m(\rho) - \sharp_f(\rho) < \sharp_{m}(\rho) +
\sharp_{m}(\sigma) - \sharp_{f}(\rho) -\sharp_{f}(\sigma) \le n.
\]
%% If \(\rho = \Free\), then \(n + 1 - 1 < n\); if \(\rho = \Malloc\),
%% then \( n - 1 + 1 < n \); if \( \rho = other\), then \( n < n
%% \). Therefore, we have \(n < n\), and then we get the contradiction.
The leftmost term \(n' + \sharp_m(\rho) - \sharp_f(\rho)\) is equal to
\(n\) for any \(\rho\).  Hence, we get contradiction.

\item Case \(P = \mu\alpha.P'\) and \(\mu\alpha.P'  \xlongrightarrow{\tau} [\mu\alpha.P'\slash\alpha]P'\)

We need to prove \(\OK_n([\mu\alpha.P' / \alpha]P')\).  Suppose not.
Then, there exists \(\sigma\) and \(Q\) such that \([\mu\alpha.P' /
  \alpha]P' \xlongrightarrow{\sigma} Q\) and \(\sharp_m(\sigma) -
\sharp_f(\sigma) > n\).  However, this contradicts to \(P
\xlongrightarrow{\tau\sigma} Q\) and \(\OK_n(P)\) as follows.
\[
n \ge \sharp_m(\tau\sigma) - \sharp_f(\tau\sigma) = \sharp_m(\sigma) -
\sharp_f(\sigma) > n.
\]

\end{itemize}
\end{proof}

\begin{pfof}{Lemma~\ref{lem:preservation}}
By induction on the derivation of \(\langle H,R,s,n, C \rangle
\xlongrightarrow{\rho} \langle H',R',s', n', C \rangle\).

\begin{itemize}

\item Case: \( \langle H, R, \scon\Sirx s, n, C \rangle
  \xlongrightarrow{\Startconst} \langle H, R, s;\Endconst, n, C\cup
  {x} \rangle \)

  We have \( \Theta; \Gamma \vdash \scon\Sirx s:P\) and \( OK_n(P)
  \). From the inversion of typing rules, we get \( \Theta; \Gamma
  \vdash s:P'' \) and \( \scon\Sirx P'' \le P \) for some \( P''
  \). By subtyping, we get \( P'';\Endconst \le Q \) and \( P
  \xLongrightarrow{\Startconst} Q \) for some \( Q \).

  we need to find \(P'\) s.t. \( \Theta; \Gamma \vdash
  s;\Endconst:P'\), \( OK_n(P')\) and \( P
  \xLongrightarrow{\Startconst} P' \). Taking \( Q \) as \( P'\), \( P
  \xLongrightarrow{\Startconst}\) and \( OK_n(P')\) hold. From \(
  \Theta; \Gamma \vdash s;\Endconst:P'';\Endconst \), \( P'';\Endconst
  \le Q \) and \rn{T-Sub}, we have \( \Theta; \Gamma \vdash
  s;\Endconst:P'\).

\item Case: \( \langle H, R, \Endconst, n, C \uplus {x} \rangle
  \xlongrightarrow{\Endconst} \langle H, R, \SKIP, n, C \rangle \)

  We have \( \Theta; \Gamma \vdash \Endconst:P\) and \( OK_n(P)
  \). From the inversion of typing rules, we get \( \Theta; \Gamma
  \vdash \Endconst:\Endconst \) and \( \Endconst \le P \). By
  subtyping, we get \( 0 \le P'' \) and \( P
  \xLongrightarrow{\Endconst} P'' \) for some \( P'' \).

  we need to find \(P'\) s.t. \( \Theta; \Gamma \vdash
  \SKIP:P'\), \( OK_n(P')\) and \( P \xLongrightarrow{\Endconst} P'
  \). Taking \( P'' \) as \( P'\), \( P \xLongrightarrow{\Endconst}
  P'\) and \( OK_n(P')\) hold. From \rn{T-Skip}, \rn{T-Sub} and \( 0
  \le P''\), we have \( \Theta; \Gamma \vdash \SKIP:P'\).

\item Case: \(\langle H, R, \FREE, n, C\rangle \xlongrightarrow{\Free}
  \langle H', R', \SKIP, n + 1, C \rangle \)

We have \(\OK_n(P)\) and \(\Theta; \Gamma \vdash \Free(x) \COL P\).
From inversion of the typing rules, we have \(\Theta; \Gamma \vdash
\Free(x) \COL \Free\) and \(\Free \le P\).  Hence, from the definition
of subtyping, we have \(\TSKIP \le P''\) and \(P
\xLongrightarrow{\Free} P''\) for some \(P''\).  We need to find
\(P'\) such that \(P \xLongrightarrow{\Free} P'\), \(\Theta; \Gamma
\vdash \SKIP \COL P'\), and \(\OK_{n+1}(P')\).  Take \(P''\) as
\(P'\).  Then, \(P \xLongrightarrow{\Free} P''\) as we stated above.
We also have \(\Theta; \Gamma \vdash \SKIP \COL P''\) from
\rn{T-Skip}, \(\TSKIP \le P''\), and \rn{T-Sub}.  \(\OK_{n+1}(P'')\)
follows from Lemma~\ref{lem:okPreserved}.

\item Case: \( \langle H, R, \LET x = \MALLOC \IN s, n, C \rangle
  \xlongrightarrow{\Malloc} \langle H', R', [x'/x]s, n - 1, C \rangle \)

From the assumption, we have \(\Theta; \Gamma \vdash \LET x = \MALLOC
\IN s \COL P\) and \(\OK_{n}(P)\). By the inversion of typing rules,
we have \(\Malloc;P_1 \le P\) and \(\Theta; \Gamma \vdash s : P_{1}\)
for some \(P_1\). We have the following derivation: \infrule{ \Malloc
  \xlongrightarrow{\Malloc} 0} {\Malloc;P_1 \xlongrightarrow{\Malloc}
  0;P_{1}} and \(0;P_1 \rightarrow P_{1}\), then we have
\(\Malloc;P_{1} \xLongrightarrow{\Malloc} P_{1}\). Hence, By the
definition of subtyping, we have \(P \xLongrightarrow{\Malloc}P''\)
and \(P_{1} \le P''\) for some \(P''\).

We need to find \(P'\) and \(\Gamma'\) such that \(\Theta; \Gamma'
\vdash [x'/x]s\COL P'\) and \(P\xLongrightarrow{\Malloc} P'\). Take
\(P''\) as \(P'\) and \([x'/x]\Gamma\) as \(\Gamma'\).  (Note that
\([x'/x]\Gamma\) is well-formed because \(x'\) is fresh.)  Then \(P
\xLongrightarrow{\Malloc} P''\) as we state above. We also have
\(\Theta;[x'/x]\Gamma \vdash [x'/x]s \COL P''\) from \rn{T-Sub},
\(\Theta;[x'/x]\Gamma \vdash [x'/x]s \COL P_1\), and \(P_1 \le P''\).
\(\OK_{n-1}(P'')\) follows from Lemma~\ref{lem:okPreserved}.

\item Case: \( \langle H, R, \SKIP;s, n, C \rangle \rightarrow \langle
  H, R, s, n, C \rangle \)

  we have \(\Theta;\Gamma \vdash \SKIP;s\COL  P\) and
  \(\OK_{n}(P)\). From the inversion of the typing rules, we have
  \(\Theta; \Gamma \vdash s\COL P_{1}\) and \(0;P_{1} \le
  P\). Hence, from the definition of subtyping, we have \(P
  \xLongrightarrow{\tau} P''\) and \(P_{1} \le P''\) for some \(P''\).

  We need to find \(P'\) such that \(\Theta; \Gamma \vdash s : P'\)
  and \(P \xLongrightarrow{\tau} P'\). Take \(P''\) as \(P'\). Then \(P
  \xLongrightarrow{\tau} P''\) as we stated above. We also have
  \(\Theta;\Gamma \vdash s\COL P''\) from \rn{T-Sub}, \(\Gamma \vdash
  s\COL P_{1}\) and \(P_{1} \le P''\). \(\OK_n(P'')\) follows from
  Lemma~\ref{lem:okPreserved}

\item Case: \( \langle H, R, *x \leftarrow y , n, C \rangle \rightarrow
  \langle H', R', \SKIP, n, C \rangle \)

  We have \(\Theta; \Gamma \vdash *x \leftarrow y : P\) and
  \(\OK_{n}(P)\). From the inversion of typing rules, we have \(0 \le
  P\).

  We need to find $P'$ such that \(\Theta; \Gamma \vdash \SKIP: P'\),
  \(P \xLongrightarrow{\tau} P'\) and \(\OK_n(P')\). Take $P$ as $P'$. Then,
  \(P \xLongrightarrow{\tau} P'\) and \(\OK_n(P')\) hold. We also have \(\Theta;
  \Gamma \vdash \SKIP: P'\) from \rn{T-Skip}, \(0 \le P\) and
  \rn{T-Sub}.

\item Case: \( \langle H, R, \LET x = y\ \IN s , n, C \rangle
  \rightarrow \langle H', R', [x'/x]s, n, C \rangle \)a

  We have \(\Theta; \Gamma \vdash \LET x = y \ \IN s \COL P\) and
  \(OK_{n}(P)\). From the inversion of typing rules, we have \(\Theta;
  \Gamma \vdash s\COL P_{1}\) and \(P_{1} \le P\).

  We need to find $P'$ and \(\Gamma'\) such that \(\Theta; \Gamma'
  \vdash [x'/x]s : P'\) , \(P \xLongrightarrow{\tau} P'\) and
  \(\OK_n(P'\)). Take \(P\) as \(P'\) and \([x'/x]\Gamma\) as
  \(\Gamma'\). Then \( P \xLongrightarrow{\tau} P'\) and \(\OK_n(P')\)
  hold.  We also have \(\Theta; \Gamma \vdash [x'/x]s\COL P\) from
  \rn{T-Sub}, \(\Theta; \Gamma \vdash [x'/x]s\COL P_{1}\) and \( P_{1}
  \le P\).

\item Case: \( \langle H, R, \LET x = \NULL \ \IN \ s, n, C\rangle
  \rightarrow \langle H', R', [x'/x]s, n, C \rangle \)

  We have \(\Theta; \Gamma \vdash \LET x = \NULL \ \IN \ s\COL P\)
  and \(OK_{n}(P)\). From the inversion of typing rules, we have
  \(\Theta; \Gamma \vdash s\COL P_{1}\) and \( P_{1} \le P\).

  We need to find $P'$ and \(\Gamma'\) such that \(\Theta; \Gamma'
  \vdash [x'/x]s\COL P'\), \(P \xLongrightarrow{\tau} P'\) and
  \(\OK_n(P')\).  Take \(P\) as \(P'\) and \([x'/x]\Gamma\) as
  \(\Gamma'\).  Then, \(P \xLongrightarrow{\tau} P'\) and
  \(\OK_n(P')\) hold.  We also have \(\Theta; \Gamma \vdash
       [x'/x]s\COL P\) from \rn{T-Sub}, \(\Theta; \Gamma \vdash
       [x'/x]s\COL P_{1}\)\( P_{1} \le P\).

\item Case: \( \langle H, R, \LET x = *y \ \IN \ s, n, C\rangle
  \rightarrow \langle H', R', [x'/x]s, n, C\rangle \)

  We have \(\Theta; \Gamma \vdash \LET x = *y \ \IN \ s\COL  P\) and
  \(OK_{n}(P)\). From the inversion of typing rules, we have \(\Theta;
  \Gamma \vdash s\COL P_{1}\) and \(P_{1} \le P\).

  We need to find \(P'\) and \(\Gamma'\) such that \(\Theta; \Gamma'
  \vdash [x'/x]s\COL P'\), \(P \xLongrightarrow{\tau} P'\) and
  \(\OK_n(P')\). Take \(P\) as \(P'\) and \([x'/x]\Gamma\) as
  \(\Gamma'\). Then, \(P \xLongrightarrow{\tau} P'\) and \(\OK_n(P')\)
  hold.  We also have \(\Theta; \Gamma' \vdash [x'/x]s\COL P\) from
  \rn{T-Sub}, \(\Theta; \Gamma' \vdash [x'/x]s\COL P_{1}\) and \(P_{1}
  \le P\).

\item Case: \(\langle H, R, \IFNULL \Sirx \ \THEN s_{1} \ \ELSE
  \ s_{2}, n, C\rangle \xlongrightarrow{\sassx} \langle H, R, s_{1}, n, C \rangle\)

  We have \(\Theta; \Gamma \vdash \IFNULL \Sirx \ \THEN \ s_{1}
  \ \ELSE \ s_{2}\COL P\) and \(\OK_{n}(P)\). From the inversion of
  typing rules, we have \(\Theta; \Gamma \vdash s_{1} : P_{1}\),
  \(\Theta; \Gamma \vdash s_{2} : P_{2}\) and \( (*x)(P_1,P_2) \le
  P\). By subtyping we get \(P \xLongrightarrow{\sassx} \) \(
  P''\)and \( P_1 \le P''\) for some \( P '' \).

  We need to find $P'$ such that \(\Theta; \Gamma \vdash s_1\COL P'\)
  , \(P \xLongrightarrow{\sassx} P'\) and \(\OK_n(P'\)).  Take \(P''\) as
  \(P'\).  Then, \(\OK_n(P')\) and \(P \xLongrightarrow{\sassx} P'\)
  hold. We also have \(\Theta; \Gamma' \vdash s_{1}\COL P'\) from
  \(\Theta; \Gamma \vdash s_{1}\COL P_1\), \(P_{1} \le P'' \) and
  \rn{T-Sub}.

\item Case: \(\langle H, R, \IFNULL \Sirx \ \THEN s_{1} \ \ELSE \ s_{2},
  n , C \rangle \xlongrightarrow{\sassxn} \langle H, R, s_{2}, n, C\rangle\).

 The proof is similar to case of  \(\langle H, R, \IFNULL \Sirx \ \THEN s_{1} \ \ELSE
  \ s_{2}, n, C \rangle \xlongrightarrow{\sassx} \langle H, R, s_{1}, n, C\rangle\).

\item Case: \( \langle H, R, f(\vec{x}) , n, C \rangle \rightarrow  \langle H, R, [\vec{x}/\vec{y}]s, n, C \rangle \)

% We have \(D(f) = s\) and \(\Theta(f) = P_1\), we have \(s \COL P_1\). 

From the inversion of \rn{T-Call}, we have \(\Theta; \Gamma \vdash
f(\vec{x}) \COL \Theta(f)\) and \(\Theta(f) \le P\).  From
\rn{Sem-Call}, we have \(D(f) = (\vec{y})s\).  From the assumption
\(\vdash D \COL \Theta\), we have \(\Theta; \vec{y} \vdash s \COL
\Theta(f)\); hence, with \(\Theta(f) \le P\), we have \(\Theta;
\vec{y} \vdash s \COL P\).  We then have \(\Theta; \vec{x} \vdash
    [\vec{x}/\vec{y}]s \COL P\) as required.

\end{itemize}
\end{pfof}  

\begin{corollary}
\label{cor:preservation}
If $OK_{n}(P)$, $\Theta; \Gamma \vdash s : P$, \(\vdash D \COL
\Theta\), and $\langle H,R,s,n,C\rangle \xlongrightarrow{\sigma}
\langle H',R',s', n', C \rangle$, then there exists $P'$ such that (1) $
\Theta; \Gamma \vdash s' : P'$, (2) \(P \xLongrightarrow{\sigma} P'\),
and (3) \(OK_{n'}(P')\).
\end{corollary}

We write \(\langle H, R, s, n \rangle \xlongrightarrow{\rho}\) if
there is a transition \(\xlongrightarrow{\rho}\) from \(\langle H, R,
s, n \rangle\).

\begin{lemma}
\label{lem:enabled}
If \(\Theta; \Gamma \vdash s \COL P\) and \(\langle H, R, s, n \rangle
\xlongrightarrow{\rho}\) and \(\rho \in \set{\Malloc, \Free, \sassx, \sassxn, \Startconst, \Endconst}\), then
there exists \(P'\) such that \(P \xLongrightarrow{\rho} P'\).
\end{lemma}

\begin{proof}
Induction on the derivation of \(\Theta; \Gamma \vdash s \COL P\).
\end{proof}

\begin{pfof}{Lemma~\ref{lem:immediateSafety}}

By contradiction.  Assume \(\langle H, R, s, n \rangle
\xlongrightarrow{\rho} \OVERFLOW\). Then, \(n\) is \(0\) and \(\rho =
\Malloc\) from \rn{Sem-OutOfMem}.  From the assumption \(\Theta;\Gamma
\vdash s \COL P\) and \(\OK_0(P)\).  From Lemma~\ref{lem:enabled},
there exists \(P'\) such that \(P \xLongrightarrow{\Malloc} P'\).
However, this contradicts \(\OK_0(P)\).


\end{pfof}


\begin{pfof}{Theorem~\ref{thm1}}

We have \(\Theta;\emptyset \vdash s\COL P, \vdash D\COL \Theta\) and
\(\OK_n(P)\).

Suppose that there exists \(\sigma\) such that \(\langle \emptyset,
\emptyset, s, n\rangle \xlongrightarrow{\sigma} \langle H', R', s',
n'\rangle \xlongrightarrow{\rho} \OVERFLOW\).  Then, \(n' = 0\) and
\(\rho = \Malloc\).  From Lemma~\ref{cor:preservation}, there exists
\(P'\) such that \(\Theta; \Gamma' \vdash s \COL P'\), \(P
\xLongrightarrow{\sigma} P'\), and \(\OK_0(P')\); hence \(\langle H',
R', s', 0\rangle \xlongrightarrow{\Malloc}\).  However, this
contradicts Lemma~\ref{lem:immediateSafety}.

\end{pfof}
